Modify the compilation scheme and the decision trees #667
The evaluation of decision trees is now not performed by decomposing the values, but by adding the position of the constructor we want to check to If statements, and the position of the subterms we want to name to Let statements.

compiler/backend/pattern_matching/pattern_matchingScript.sml
@@ -10,13 +10,48 @@ Definition of terms
 Every term is a constructor with 0 or more arguments
 Constructors are identified by num
 *)
-Datatype `term = Term num (term list)`;
+Datatype:
+  term = Term num (term list)
+End
+
+(*
+A position describes a path to a sub-term in a term
+*)
+Datatype:
+  position =
+    EmptyPos
+  | Pos num position
+End
+
+Definition app_pos_def:
+  (app_pos EmptyPos p = p) /\
+  (app_pos (Pos 0 pos) (Term c (x::xs)) =
+    app_pos pos x) /\
+  (app_pos (Pos (SUC n) pos) (Term c (x::xs)) =
+    app_pos (Pos n pos) (Term c xs))
+End
+
+Definition snoc_pos_def:
+  (snoc_pos n EmptyPos = (Pos n EmptyPos)) /\
+  (snoc_pos n (Pos m pos) = (Pos m (snoc_pos n pos)))
+End
+
+(* a list position describes a path to a sub-term in a list of term *)
+Type listPos = ``:(num # position)``
+
+Definition app_list_pos_def:
+  (app_list_pos (0, pos) (x::xs) =
+    app_pos pos x) /\
+  (app_list_pos (SUC n, pos) (x::xs) =
+    app_list_pos (n, pos) xs)
+End
 
 (*
 Definition of full patterns with as clauses
 Variables are identified by num
 *)
-Datatype `pat =
+Datatype:
+  pat =
     Any
   | Var num
   (* A constructor pattern is an constructor id, the number of constructors
@@ -24,14 +59,13 @@ Datatype `pat =
   | Cons num num (pat list)
   | Or pat pat
   | As pat num (* (p:pat) as (x:num) *)
-`;
+End
 
 (*
 We parametrize the size function by an arity a to take into account the fact
 that a Any or a Var can be expanded into a list of Any patterns
 *)
 Definition psize_def:
-  (* (psize a Any = ((2:num) ** (a+2)) + 1) /\ *)
   (psize a Any = (2:num) ** (2 ** a)) /\
   (psize a (Var n) = (2 ** (2 ** a))) /\
   (psize a (Cons n t []) = 2 + a) /\
@@ -44,7 +78,9 @@ End
 Represent a branch (p => e) in a match expression
 the result expression is just a number for now
 *)
-Datatype `branch = Branch (pat list) num`;
+Datatype:
+  branch = Branch (pat list) num
+End
 
 Definition patterns_def:
   patterns (Branch ps e) = ps
@@ -55,12 +91,33 @@ Definition expr_def:
 End
 
 (* pattern matrix *)
-val _ = type_abbrev("patmat", ``:branch list``)
+Type patmat = ``:branch list``
 
 (* Invariant of pattern matrices *)
-Definition inv_mat_def:
-  inv_mat m = ?n. EVERY (\l. (LENGTH (patterns l)) = n) m
+Definition inv_mat_aux_def:
+  (inv_mat [] = T) /\
+  (inv_mat [x] = T) /\
+  (inv_mat ((Branch l1 e1)::(Branch l2 e2)::m) =
+    ((LENGTH l1 = LENGTH l2) /\ (inv_mat ((Branch l2 e2)::m))))
 End
+
+Theorem inv_mat_def:
+  !m. inv_mat m = ?n. EVERY (\l. (LENGTH (patterns l)) = n) m
+Proof
+  Induct_on `m`
+  >- (rw[] \\ fs[inv_mat_aux_def])
+  >- (rw[] \\ EQ_TAC \\ rw[]
+      >- (Cases_on `m`
+          >- fs[inv_mat_aux_def]
+	  >- (Cases_on `h` \\
+              Cases_on `h'` \\
+              fs[inv_mat_aux_def, patterns_def]))
+      >- (Cases_on `m`
+          >- fs[inv_mat_aux_def]
+	  >- (Cases_on `h` \\
+              Cases_on `h'` \\
+              fs[inv_mat_aux_def, patterns_def])))
+QED;
 
 Theorem inv_mat_dcmp:
   !b m. inv_mat (b::m) ==> inv_mat m
@@ -267,7 +324,7 @@ Proof
 QED;
 
 (* Semantics of matching *)
-val pmatch_def = tDefine "match_def" `
+Definition pmatch_def:
   (pmatch Any  t = T) /\
   (pmatch (Var n) t = T) /\
   (pmatch (Cons pcons _ pargs) (Term tcons targs) =
@@ -280,7 +337,8 @@ val pmatch_def = tDefine "match_def" `
     ((pmatch p t) /\
      (pmatch (Cons pcons tinfo ps) (Term tcons ts)))) /\
   (pmatch (Or p1 p2) t = ((pmatch p1 t) \/ (pmatch p2 t))) /\
-  (pmatch (As p num) t = pmatch p t)`
+  (pmatch (As p num) t = pmatch p t)
+Termination
   (WF_REL_TAC `measure (\ (x,_). psize 1 x)` \\ rw[psize_def] \\
   Induct_on `pargs`
   >- fs[psize_def]
@@ -288,15 +346,16 @@ val pmatch_def = tDefine "match_def" `
       fs[MEM]
       >- (fs[psize_def] \\
           `0 < psize 1 (Cons pcons' v0 pargs) ` by fs[psize_gt_zero] \\
-	  `(psize 1 h) <= ((psize 1 h) * (psize 1 (Cons pcons' v0 pargs)))` by
-	  fs[LE_MULT_CANCEL_LBARE] \\
-	  decide_tac)
+          `(psize 1 h) <= ((psize 1 h) * (psize 1 (Cons pcons' v0 pargs)))` by
+          fs[LE_MULT_CANCEL_LBARE] \\
+          decide_tac)
       >- (res_tac \\
           fs[psize_def] \\
           `0 < psize 1 h ` by fs[psize_gt_zero] \\
           `psize 1 (Cons pcons' v0 pargs) <= (psize 1 h) * (psize 1 (Cons pcons' v0 pargs))` by
           fs[] \\
-	  decide_tac)))
+          decide_tac)))
+End
 
 Definition pmatch_list_def:
   (pmatch_list [] [] = T) /\
@@ -700,10 +759,10 @@ Proof
   >- (Cases_on `m` \\
       Cases_on `c = pcons'`
       >- fs[spec_def, msize_def, n_any_length, ars_inv_def,
-	    ars_branch_def, ars_pat_def]
+            ars_branch_def, ars_pat_def]
       >- fs[spec_def]
       >- fs[spec_def, msize_def, n_any_length, ars_inv_def,
-	    ars_branch_def, ars_pat_def]
+            ars_branch_def, ars_pat_def]
       >- (fs[spec_def, msize_def, ars_inv_def, inv_mat_dcmp, inv_mat_def] \\
           Cases_on `h` \\
           fs[patterns_def, msize_def]))
@@ -712,17 +771,17 @@ Proof
           >- (imp_res_tac ars_inv_or1 \\
               imp_res_tac inv_mat_or1 \\
               fs[])
-	  >- (Cases_on `spec c a [Branch (p1::ps) e] = []`
+          >- (Cases_on `spec c a [Branch (p1::ps) e] = []`
               >- (fs[msize_app2] \\
                   imp_res_tac ars_inv_or2 \\
                   imp_res_tac inv_mat_or2 \\
                   fs[])
-	      >- (fs[msize_app] \\
+              >- (fs[msize_app] \\
                   imp_res_tac ars_inv_or1 \\
                   imp_res_tac inv_mat_or1 \\
                   fs[])))
       >- (fs[spec_def, msize_def, msize_app]
-	  >- (imp_res_tac ars_inv_or1 \\
+          >- (imp_res_tac ars_inv_or1 \\
               imp_res_tac inv_mat_or1 \\
               imp_res_tac inv_mat_cons \\
               imp_res_tac ars_inv_cons \\
@@ -922,13 +981,20 @@ Proof
 QED;
 
 (* definition of decision trees *)
-Datatype `dTree =
+Datatype:
+  dTree =
     Leaf num
   | Fail
   | Swap num dTree
-  | If num dTree dTree
+  (*
+     If pos c a dt1 dt2
+     if value at position pos has constructor c
+     and a arguments, then go to decision tree
+     dt1 else go to decision tree dt2
+  *)
+  | If listPos num num dTree dTree
   | Let num dTree
-`;
+End
 
 (* Swap the first and ith items in a list *)
 Definition get_ith_def:
@@ -994,21 +1060,14 @@ End
 Definition dt_eval_def:
   (dt_eval ts (Leaf k) = k) /\
   (dt_eval ts (Swap i dt) = dt_eval (swap_items i ts) dt) /\
-  (dt_eval ((Term c targs)::ts) (If c' dt1 dt2) =
-    if c = c'
-    then dt_eval (targs++ts) dt1
-    else dt_eval (targs++ts) dt2) /\
+  (dt_eval ts (If pos c' a dt1 dt2) =
+    case (app_list_pos pos ts) of
+      (Term c targs) =>
+        (if c = c' /\ (LENGTH targs) = a
+         then dt_eval ts dt1
+         else dt_eval ts dt2)) /\
   (dt_eval ts (Let k dt) = dt_eval ts dt)
 End
-
-(* Definition of occurences and their application to terms *)
-(* val _ = type_abbrev("occurences", ``:num list``) *)
-
-(* Definition occur_term_def: *)
-(*   (occur_term t [] = t) /\ *)
-(*   (occur_term (Term tcons targs) (occ::os) = *)
-(*     occur_term (get_ith occ targs) os) *)
-(* End *)
 
 Definition all_wild_or_vars_def:
   (all_wild_or_vars [] = T) /\
@@ -1095,15 +1154,15 @@ containing pairs of constructors, expected number of constructors for a type,
 an arity for the constructor, and list of identifiers to be bound for each of
 these constructors
 *)
-val _ = type_abbrev("cons_infos", ``:((num # num # num # (num list)) list)``)
-val _ = type_abbrev("col_infos", ``:(num list) # cons_infos``)
+Type cons_infos = ``:((num # num # num # (num list)) list)``
+Type col_infos = ``:(num list) # cons_infos``
 
 (* Add an indentifier to the "default" identifiers *)
 Definition add_def_id_def:
   add_def_id id (ids, cinfos) = (id::ids, cinfos)
 End
 
-(* Add a constructor to the list of constructors of the column *)
+(* Adds an identifier associated with the constructor c *)
 Definition add_cons_id_aux_def:
   (add_cons_id_aux c n a id ([]: cons_infos) = [(c,n,a,[id])]) /\
   (add_cons_id_aux c n a id ((c', n', a', cids)::cinfos) =
@@ -1117,7 +1176,7 @@ Definition add_cons_id_def:
     (ids, (add_cons_id_aux c n a id cinfos)))
 End
 
-(* Adds an identifier associated with the constructor c *)
+(* Add a constructor to the list of constructors of the column *)
 Definition add_cons_aux_def:
   (add_cons_aux c n a [] = [(c,n,a,[])]) /\
   (add_cons_aux c n a ((c', n', a', cids)::cinfos) =
@@ -1185,7 +1244,7 @@ End
 Definition get_cons_in_def:
   (get_cons_in Any = []) /\
   (get_cons_in (Var _) = []) /\
-  (get_cons_in (Cons c _ sub_pats) = [(c, (LENGTH sub_pats))]) /\
+  (get_cons_in (Cons c _ spats) = [(c, (LENGTH spats))]) /\
   (get_cons_in (Or p1 p2) = merge_list (get_cons_in p1)
                                        (get_cons_in p2)) /\
   (get_cons_in (As p _) = get_cons_in p)
@@ -1215,13 +1274,11 @@ Definition col_infos_def:
   (col_infos ((Branch ((As p n)::ps) e)::rs) =
     if all_wild_or_vars [As p n]
     then add_def_id n (add_def_bindings p (col_infos rs))
-    else FOLDL (\infos (cons, arity). add_cons_bindings cons (get_nb_types p) arity p infos)
+    else FOLDL (\infos (cons, arity).
+                 add_cons_id cons (get_nb_types p) arity n
+                   (add_cons_bindings cons (get_nb_types p) arity p infos))
                (col_infos rs)
                (get_cons_in p))
-End
-
-Definition cinfo_size_def:
-  cinfo_size (_,cons) = LENGTH cons
 End
 
 (* Tell if the patterns contain all the constructors of a signature
@@ -1238,7 +1295,7 @@ Definition add_bindings_from_ids_def:
   (add_bindings_from_ids (id::ids) dt = Let id (add_bindings_from_ids ids dt))
 End
 
-(* The new attempt : couting the number of constructors *)
+(* Counting the number of constructors to prove termination *)
 Definition nb_cons_pat_def:
   (nb_cons_pat Any = (1:num)) /\
   (nb_cons_pat (Var _) = 1) /\
@@ -1346,7 +1403,7 @@ Proof
           imp_res_tac msize_inv_gt_zero \\
           imp_res_tac inv_mat_dcmp \\
           fs[default_def, nb_cons_def, nb_cons_branch_def, nb_cons_pat_def,
-	     nb_cons_app]))
+             nb_cons_app]))
   >- (Cases_on `rs`
       >- (fs[default_def, nb_cons_def, nb_cons_branch_def] \\
           `msize [Branch (p::ps) e] > 0` by fs[msize_def] \\
@@ -1354,7 +1411,7 @@ Proof
           fs[nb_cons_pat_def])
       >- (fs[default_def, nb_cons_def, nb_cons_branch_def, nb_cons_pat_def] \\
           `msize (Branch (p::ps) e::h::t) > 0` by fs[msize_def] \\
-	  imp_res_tac inv_mat_as \\
+          imp_res_tac inv_mat_as \\
           fs[]))
   >- fs[msize_def]
 QED;
@@ -1370,14 +1427,14 @@ Proof
   >- (Cases_on `m`
       >- fs[is_cons_fcol_def, is_cons_fcol_branch_def, is_cons_fcol_pat_def]
       >- (fs[is_cons_fcol_def, is_cons_fcol_branch_def, nb_cons_pat_def,
-	     is_cons_fcol_pat_def, nb_cons_def, nb_cons_branch_def, default_def] \\
+             is_cons_fcol_pat_def, nb_cons_def, nb_cons_branch_def, default_def] \\
           imp_res_tac msize_inv_gt_zero \\
           imp_res_tac inv_mat_dcmp \\
           fs[]))
   >- (Cases_on `m`
       >- fs[is_cons_fcol_def, is_cons_fcol_branch_def, is_cons_fcol_pat_def]
       >- (fs[is_cons_fcol_def, is_cons_fcol_branch_def, nb_cons_pat_def,
-	     is_cons_fcol_pat_def, nb_cons_def, nb_cons_branch_def, default_def] \\
+             is_cons_fcol_pat_def, nb_cons_def, nb_cons_branch_def, default_def] \\
           imp_res_tac msize_inv_gt_zero \\
           imp_res_tac inv_mat_dcmp \\
           fs[]))
@@ -1401,18 +1458,18 @@ Proof
               fs[])))
   >- (Cases_on `m`
       >- (fs[default_def, nb_cons_def, nb_cons_branch_def, nb_cons_pat_def,
-	     nb_cons_app] \\
+             nb_cons_app] \\
           `msize [Branch (p1::ps) e] > 0` by fs[msize_def]  \\
           `msize [Branch (p2::ps) e] > 0` by fs[msize_def]  \\
           imp_res_tac inv_mat_or1 \\
           imp_res_tac inv_mat_or2 \\
           imp_res_tac nb_cons_default_aux \\
           rfs[nb_cons_def, nb_cons_branch_def, is_cons_fcol_def,
-	      is_cons_fcol_branch_def, nb_cons_pat_def,
-	      is_cons_fcol_pat_def]  \\
+              is_cons_fcol_branch_def, nb_cons_pat_def,
+              is_cons_fcol_pat_def]  \\
           fs[])
       >- (fs[default_def, nb_cons_def, nb_cons_branch_def, nb_cons_pat_def,
-	     nb_cons_app] \\
+             nb_cons_app] \\
           `msize [Branch (p1::ps) e] > 0` by fs[msize_def]  \\
           `msize [Branch (p2::ps) e] > 0` by fs[msize_def]  \\
           imp_res_tac inv_mat_or1 \\
@@ -1422,17 +1479,17 @@ Proof
           imp_res_tac msize_inv_gt_zero \\
           imp_res_tac nb_cons_default_aux \\
           fs[nb_cons_def, nb_cons_branch_def, is_cons_fcol_def,
-	      is_cons_fcol_branch_def, nb_cons_pat_def,
-	      is_cons_fcol_pat_def] \\
+              is_cons_fcol_branch_def, nb_cons_pat_def,
+              is_cons_fcol_pat_def] \\
           rfs[] \\ fs[]))
   >- (Cases_on `rs`
       >- (fs[default_def, nb_cons_def, nb_cons_branch_def, nb_cons_pat_def,
-	     is_cons_fcol_def, is_cons_fcol_branch_def, is_cons_fcol_pat_def] \\
+             is_cons_fcol_def, is_cons_fcol_branch_def, is_cons_fcol_pat_def] \\
           imp_res_tac inv_mat_as \\
           `msize [Branch (p::ps) e] > 0` by fs[msize_def] \\
           fs[])
       >- (fs[default_def, nb_cons_def, nb_cons_branch_def, nb_cons_pat_def,
-	     is_cons_fcol_def, is_cons_fcol_branch_def, is_cons_fcol_pat_def] \\
+             is_cons_fcol_def, is_cons_fcol_branch_def, is_cons_fcol_pat_def] \\
           imp_res_tac inv_mat_as \\
           `msize (Branch (p::ps) e::h::t) > 0` by fs[msize_def] \\
           fs[]))
@@ -1473,22 +1530,22 @@ Proof
   ho_match_mp_tac (theorem "spec_ind") \\ rw[]
   >- (Cases_on `m`
       >- fs[spec_def, nb_cons_def, nb_cons_branch_def, nb_cons_pat_def,
-	    nb_cons_branch_app, nb_cons_branch_n_any]
+            nb_cons_branch_app, nb_cons_branch_n_any]
       >- (fs[spec_def, nb_cons_def, nb_cons_branch_def, nb_cons_pat_def,
-	    nb_cons_branch_app, nb_cons_branch_n_any] \\
+            nb_cons_branch_app, nb_cons_branch_n_any] \\
           imp_res_tac inv_mat_dcmp \\
           imp_res_tac msize_inv_gt_zero \\
           fs[nb_cons_def, nb_cons_branch_app, nb_cons_branch_def, nb_cons_branch_n_any,
-	     nb_cons_pat_def]))
+             nb_cons_pat_def]))
   >- (Cases_on `m`
       >- fs[spec_def, nb_cons_def, nb_cons_branch_def, nb_cons_pat_def,
-	    nb_cons_branch_app, nb_cons_branch_n_any]
+            nb_cons_branch_app, nb_cons_branch_n_any]
       >- (fs[spec_def, nb_cons_def, nb_cons_branch_def, nb_cons_pat_def,
-	    nb_cons_branch_app, nb_cons_branch_n_any] \\
+            nb_cons_branch_app, nb_cons_branch_n_any] \\
           imp_res_tac inv_mat_dcmp \\
           imp_res_tac msize_inv_gt_zero \\
           fs[nb_cons_def, nb_cons_branch_app, nb_cons_branch_def, nb_cons_branch_n_any,
-	     nb_cons_pat_def]))
+             nb_cons_pat_def]))
   >- (Cases_on `m` \\ Cases_on `c=pcons'` \\
       fs[spec_def, nb_cons_def, nb_cons_branch_app, nb_cons_branch_def]
       >- (`0 < nb_cons_branch ps` by fs[nb_cons_branch_gt_zero] \\
@@ -1532,7 +1589,7 @@ Proof
           fs[nb_cons_pat_def])
       >- (fs[spec_def, nb_cons_def, nb_cons_branch_def, nb_cons_pat_def] \\
           `msize (Branch (p::ps) e::h::t) > 0` by fs[msize_def] \\
-	  imp_res_tac inv_mat_as \\
+          imp_res_tac inv_mat_as \\
           fs[]))
   >- fs[msize_def]
 QED;
@@ -1551,14 +1608,14 @@ Proof
           imp_res_tac inv_mat_dcmp \\
           imp_res_tac msize_inv_gt_zero \\
           fs[nb_cons_def, nb_cons_branch_app, nb_cons_branch_def, nb_cons_branch_n_any,
-	     nb_cons_pat_def]))
+             nb_cons_pat_def]))
   >- (Cases_on `m`
       >- fs[spec_def, is_cons_fcol_def, is_cons_fcol_branch_def, is_cons_fcol_pat_def]
       >- (fs[spec_def, is_cons_fcol_def, is_cons_fcol_branch_def, is_cons_fcol_pat_def] \\
           imp_res_tac inv_mat_dcmp \\
           imp_res_tac msize_inv_gt_zero \\
           fs[nb_cons_def, nb_cons_branch_app, nb_cons_branch_def, nb_cons_branch_n_any,
-	     nb_cons_pat_def]))
+             nb_cons_pat_def]))
   >- (Cases_on `m`
       >- (Cases_on `c=pcons'`
           >- (fs[spec_def, nb_cons_def, nb_cons_branch_app, nb_cons_branch_def] \\
@@ -1595,23 +1652,23 @@ Proof
               rpt (first_x_assum (qspecl_then [`c`,`a`] assume_tac)) \\
               Cases_on `nb_cons (spec c a (h::t)) = nb_cons (h::t)`
               >- fs[nb_cons_branch_gt_zero, nb_cons_gt_zero, LESS_MULT2]
-	      >- (`nb_cons (spec c a (h::t)) < nb_cons (h::t)` by fs[] \\
+              >- (`nb_cons (spec c a (h::t)) < nb_cons (h::t)` by fs[] \\
                   fs[]))))
   >- (Cases_on `m`
       >- (fs[spec_def, nb_cons_def, nb_cons_branch_def, nb_cons_pat_def,
-	     nb_cons_app] \\
+             nb_cons_app] \\
           `msize [Branch (p1::ps) e] > 0` by fs[msize_def]  \\
           `msize [Branch (p2::ps) e] > 0` by fs[msize_def]  \\
           imp_res_tac inv_mat_or1 \\
           imp_res_tac inv_mat_or2 \\
           imp_res_tac nb_cons_spec_aux \\
           rfs[nb_cons_def, nb_cons_branch_def, is_cons_fcol_def,
-	      is_cons_fcol_branch_def, nb_cons_pat_def,
-	      is_cons_fcol_pat_def]  \\
+              is_cons_fcol_branch_def, nb_cons_pat_def,
+              is_cons_fcol_pat_def]  \\
           rpt (first_x_assum (qspecl_then [`c`,`a`] assume_tac)) \\
           fs[])
       >- (fs[spec_def, nb_cons_def, nb_cons_branch_def, nb_cons_pat_def,
-	     nb_cons_app] \\
+             nb_cons_app] \\
           `msize [Branch (p1::ps) e] > 0` by fs[msize_def]  \\
           `msize [Branch (p2::ps) e] > 0` by fs[msize_def]  \\
           imp_res_tac inv_mat_or1 \\
@@ -1621,19 +1678,19 @@ Proof
           imp_res_tac msize_inv_gt_zero \\
           imp_res_tac nb_cons_spec_aux \\
           fs[nb_cons_def, nb_cons_branch_def, is_cons_fcol_def,
-	      is_cons_fcol_branch_def, nb_cons_pat_def,
-	      is_cons_fcol_pat_def] \\
+              is_cons_fcol_branch_def, nb_cons_pat_def,
+              is_cons_fcol_pat_def] \\
           rfs[] \\
           rpt (first_x_assum (qspecl_then [`c`,`a`] assume_tac)) \\
           fs[]))
   >- (Cases_on `rs`
       >- (fs[spec_def, nb_cons_def, nb_cons_branch_def, nb_cons_pat_def,
-	     is_cons_fcol_def, is_cons_fcol_branch_def, is_cons_fcol_pat_def] \\
+             is_cons_fcol_def, is_cons_fcol_branch_def, is_cons_fcol_pat_def] \\
           imp_res_tac inv_mat_as \\
           `msize [Branch (p::ps) e] > 0` by fs[msize_def] \\
           fs[])
       >- (fs[spec_def, nb_cons_def, nb_cons_branch_def, nb_cons_pat_def,
-	     is_cons_fcol_def, is_cons_fcol_branch_def, is_cons_fcol_pat_def] \\
+             is_cons_fcol_def, is_cons_fcol_branch_def, is_cons_fcol_pat_def] \\
           imp_res_tac inv_mat_as \\
           `msize (Branch (p::ps) e::h::t) > 0` by fs[msize_def] \\
           fs[]))
@@ -1672,8 +1729,8 @@ Proof
   fs[swap_items_def] \\
   Cases_on `t` \\
   fs[swap_items_def] \\
-  rw[max_a_branch_def, get_ith_def, replace_ith_droptake] \\
-  fs[LENGTH_APPEND, LENGTH_TAKE_EQ, TAKE_LENGTH_ID_rwt, max_a_app] \\
+  rw[get_ith_def, replace_ith_droptake] \\
+  fs[LENGTH_APPEND, LENGTH_TAKE_EQ, TAKE_LENGTH_ID_rwt] \\
   Cases_on `i-1`
   >- fs[nb_cons_def, nb_cons_branch_def]
   >- (fs[DROP_def, nb_cons_branch_def, nb_cons_branch_app] \\
@@ -1704,100 +1761,127 @@ Proof
           first_x_assum (qspec_then `msize (Branch l n::h::t)` assume_tac) \\
           fs[] \\
           imp_res_tac inv_mat_dcmp \\
-          res_tac \\
+           res_tac \\
           fs[msize_def, nb_cons_branch_swap]))
 QED;
+
+Definition pos_default_def:
+  (pos_default (p::pos) = pos)
+End
+
+Definition pos_spec_aux_def:
+  (pos_spec_aux a n p =
+    GENLIST (λx. (n, snoc_pos x p)) a)
+End
+
+Definition pos_spec_def:
+  (pos_spec a ((n,p)::pos) =
+    (pos_spec_aux a n p) ++ pos)
+End
 
 (* compilation scheme a pattern matrix to a decision tree
    based on a heuristic h *)
 Definition compile_def:
-  (compile h [] useh = Fail) /\
-  (compile h ((Branch [] e)::bs) useh = Leaf e) /\
-  (compile h ((Branch ps e)::bs) useh =
+  (compile h pos [] useh = Fail) /\
+  (compile h pos ((Branch [] e)::bs) useh = Leaf e) /\
+  (compile h pos ((Branch ps e)::bs) useh =
     if ~(inv_mat ((Branch ps e)::bs)) then ARB else
     if all_wild_or_vars ps
-    then (add_bindings ps (Leaf e))
+    then Leaf e
     else
       (* we select a column using heuristic h *)
       let sel_col = (h ((Branch ps e)::bs)) in
       if ((sel_col > 0) /\ (sel_col < (msize ((Branch ps e)::bs))) /\ useh)
-      then Swap sel_col (compile h (swap_columns sel_col ((Branch ps e)::bs)) F)
+      then Swap sel_col (compile h pos (swap_columns sel_col ((Branch ps e)::bs)) F)
       else (if (is_cons_fcol ((Branch ps e)::bs)) then
             (let cinfos = col_infos ((Branch ps e)::bs) in
              if (is_col_complete cinfos)
-             then make_complete h ((Branch ps e)::bs) cinfos
-             else make_partial h ((Branch ps e)::bs) cinfos) else ARB)) /\
-  (make_complete h m (defs,(c,_,a,binds)::[]) =
+             then make_complete h pos ((Branch ps e)::bs) cinfos
+             else make_partial h pos ((Branch ps e)::bs) cinfos) else ARB)) /\
+  (make_complete h pos m (defs,(c,_,a,binds)::[]) =
     if inv_mat m /\ (msize m) > 0 /\ m <> [] /\ is_cons_fcol m then
-     (add_bindings_from_ids defs
-      (add_bindings_from_ids binds
-       (compile h (spec c a m) T)))
+       (compile h (pos_spec a pos) (spec c a m) T)
     else ARB) /\
-  (make_complete h m (defs,(c,_,a,binds)::cons) =
+  (make_complete h pos m (defs,(c,_,a,binds)::cons) =
     if inv_mat m /\ (msize m) > 0 /\ m <> [] /\ is_cons_fcol m then
-    If c (add_bindings_from_ids defs
-          (add_bindings_from_ids binds
-           (compile h (spec c a m) T)))
-         (make_complete h m (defs, cons))
+    If (HD pos) c a (compile h (pos_spec a pos) (spec c a m) T)
+           (make_complete h pos m (defs, cons))
     else ARB) /\
-  (make_partial h m (defs,[]) =
+  (make_partial h pos m (defs,[]) =
     if inv_mat m /\ (msize m) > 0 /\ m <> [] /\ is_cons_fcol m then
-    add_bindings_from_ids defs
-      (compile h (default m) T)
+      (compile h (pos_default pos) (default m) T)
     else ARB) /\
-  (make_partial h m (defs,(c,_,a,binds)::cons) =
+  (make_partial h pos m (defs,(c,_,a,binds)::cons) =
     if inv_mat m /\ (msize m) > 0 /\ m <> [] /\ is_cons_fcol m then
-    If c (add_bindings_from_ids defs
-          (add_bindings_from_ids binds
-           (compile h (spec c a m) T)))
-         (make_partial h m (defs, cons))
+    If (HD pos) c a (compile h (pos_spec a pos) (spec c a m) T)
+           (make_partial h pos m (defs, cons))
     else ARB)
 Termination
 WF_REL_TAC `(inv_image ($< LEX ($< LEX $<))
-            (\x. case x of INL(_,m,b) => (nb_cons m, (1:num), if b then (1:num) else 0)
-                         | INR y => (case y of INL(_,m,_,i) =>
+            (\x. case x of INL(_,_,m,b) => (nb_cons m, (1:num), if b then (1:num) else 0)
+                         | INR y => (case y of INL(_,_,m,_,i) =>
                                       (nb_cons m, (0:num), LENGTH i)
-                                     | INR(_,m,_,i) =>
+                                     | INR(_,_,m,_,i) =>
                                       (nb_cons m, (0:num), LENGTH i))))` \\
 rw[]
->- (`col_infos (Branch (v12::v13) e::bs) = (p_1, p_2)` by fs[] \\
-    fs[])
->- (`col_infos (Branch (v12::v13) e::bs) = (p_1, p_2)` by fs[] \\
-    fs[])
->- (`col_infos (Branch (v12::v13) e::bs) = (p_1, p_2)` by fs[] \\
-    fs[])
->- (`col_infos (Branch (v12::v13) e::bs) = (p_1, p_2)` by fs[] \\
-    fs[])
->- (`col_infos (Branch (v12::v13) e::bs) = (p_1, p_2)` by fs[] \\
-    fs[])
->- (`col_infos (Branch (v12::v13) e::bs) = (p_1, p_2)` by fs[] \\
-    fs[])
->- (DISJ2_TAC \\ fs[nb_cons_swap])
 >- imp_res_tac nb_cons_default
 >- (imp_res_tac nb_cons_spec \\
     first_x_assum (qspecl_then [`c`, `a`] assume_tac) \\
     fs[])
+>- (`col_infos (Branch (v14::v15) e::bs) = (p_1, p_2)` by fs[] \\
+    fs[])
+>- (`col_infos (Branch (v14::v15) e::bs) = (p_1, p_2)` by fs[] \\
+    fs[])
+>- (`col_infos (Branch (v14::v15) e::bs) = (p_1, p_2)` by fs[] \\
+    fs[])
+>- (`col_infos (Branch (v14::v15) e::bs) = (p_1, p_2)` by fs[] \\
+    fs[])
+>- (`col_infos (Branch (v14::v15) e::bs) = (p_1, p_2)` by fs[] \\
+    fs[])
+>- (`col_infos (Branch (v14::v15) e::bs) = (p_1, p_2)` by fs[] \\
+    fs[])
+>- (DISJ2_TAC \\ fs[nb_cons_swap])
 >- (imp_res_tac nb_cons_spec \\
     first_x_assum (qspecl_then [`c`, `a`] assume_tac) \\
     fs[])
 End
 
+Definition initial_pos_def:
+  (initial_pos (width:num) =
+    GENLIST (λx. (x, EmptyPos)) width)
+End
+
+(* Experiments *)
+Definition dumb_heuristic_def:
+  (dumb_heuristic m =
+    if (is_cons_fcol m) \/ (m = []) \/ (msize m = 0) then (0:num)
+    else 1 + (dumb_heuristic (remove_fst_col m)))
+Termination
+  WF_REL_TAC `measure (\m. msize m)` \\ rw[] \\
+  Cases_on `m` \\
+  fs[msize_def, is_cons_fcol_def] \\
+  Cases_on `h` \\ Cases_on `l` \\
+  fs[remove_fst_col_def, msize_def]
+End
+
+EVAL ``compile dumb_heuristic (initial_pos 1) [(Branch [As (Cons 1 2 [Var 5; Cons 2 0 []]) 1] 10); (Branch [As (Cons 1 2 [Var 5; Var 6]) 2] 11)] T``
+
 Theorem compile_complete:
-  (!c h m useh v k. (msize m) = (LENGTH v) /\
-                    useh /\
-                    c > (3 * (LENGTH m) * (msize m) + 1) ==>
+  (!h m useh v k. (msize m) = (LENGTH v) /\
+                  (inv_mat m) /\
+                  useh ==>
+                  ((match m v = SOME k) ==>
+                  (dt_eval v (compile h m useh) = k))) /\
+  (!h m cinfos v k. (msize m) = (LENGTH v) /\
+                    (inv_mat m) /\
+                    (is_col_complete cinfos) ==>
                     ((match m v = SOME k) ==>
-                    (dt_eval v (compile c h m useh) = k))) /\
-  (!c h m cinfos v k. (msize m) = (LENGTH v) /\
-                      c > (3 * (LENGTH m) * (msize m)) /\
-                      (is_col_complete cinfos) ==>
-                      ((match m v = SOME k) ==>
-                       (dt_eval v (make_complete c h m cinfos) = k))) /\
-  (!c h m cinfos v k. (msize m) = (LENGTH v) /\
-                      c > (3 * (LENGTH m) * (msize m)) /\
-                      ~(is_col_complete cinfos) ==>
-                      ((match m v = SOME k) ==>
-                       (dt_eval v (make_partial c h m cinfos) = k)))
+                    (dt_eval v (make_complete h m cinfos) = k))) /\
+  (!h m cinfos v k. (msize m) = (LENGTH v) /\
+                    (inv_mat m) /\
+                    ~(is_col_complete cinfos) ==>
+                    ((match m v = SOME k) ==>
+                    (dt_eval v (make_partial h m cinfos) = k)))
 Proof
   ho_match_mp_tac (theorem "compile_ind") \\ rw[]
   >- fs[match_def]
@@ -1806,16 +1890,16 @@ Proof
       fs[pmatch_list_def, dt_eval_def])
   >- (fs[compile_def] \\
       Cases_on `v` \\ fs[msize_def] \\
-      Cases_on `all_wild_or_vars (v14::v15)` \\ fs[]
+      Cases_on `all_wild_or_vars (v12::v13)` \\ fs[]
       >- (fs[match_def] \\
-          `LENGTH (h::t) = LENGTH (v14::v15)` by fs[] \\
+          `LENGTH (h::t) = LENGTH (v12::v13)` by fs[] \\
           imp_res_tac all_wild_vars_pmatch_list \\
           fs[eval_add_bindings, dt_eval_def])
       >- cheat)
       (*
       >- (Cases_on `h (Branch (v12::v13) e::bs) > 0` \\ fs[]
           >- (fs[swap_columns_length, swap_columns_msize, msize_def,
-		 dt_eval_def]
+                 dt_eval_def]
               `SUC`*)
   >- (fs[compile_def] \\
       (* we must show that add_bindings_from_id doesn't effect evaluation *)
